specs/ecc/Spec.EC.Projective.fst
@@ -18,7 +18,7 @@ let is_point_at_inf (k:curve) (p:proj_point k) =
 
 
 let to_proj_point (k:curve) (p:aff_point k) : proj_point k =
-  let (x, y) = p in (x, y, one k)
+  let (x, y) = p in if is_aff_point_at_inf k p then point_at_inf k else (x, y, one k)
 
 let to_aff_point (k:curve) (p:proj_point k) : aff_point k =
   // if is_proj_point_at_inf p then aff_point_at_inf
@@ -28,11 +28,28 @@ let to_aff_point (k:curve) (p:proj_point k) : aff_point k =
   let y = fmul k py zinv in
   (x, y)
 
-// is_on_curve k (to_aff_point k p) \/ is_point_at_inf k p
+// if aff_point_inv k (to_aff_point k p)
+// then is_point_at_inf (px, py, pz) = (pz = 0 \/ (px = 0 && py = 0))
 let point_inv (k:curve) (p:proj_point k) =
-  aff_point_inv k (to_aff_point k p)
+  is_on_curve k (to_aff_point k p) \/ is_point_at_inf k p
 
 let proj_point_c (k:curve) = p:proj_point k{point_inv k p}
+
+
+let to_aff_point_c (k:curve) (p:proj_point_c k) : aff_point_c k =
+  let (px, py, pz) = p in
+  if is_point_at_inf k p then begin
+    Lib.NatMod.lemma_pow_mod #k.prime pz (k.prime - 2);
+    Lib.NatMod.lemma_pow_zero (k.prime - 2);
+    assert (to_aff_point k p == aff_point_at_inf k) end;
+  to_aff_point k p
+
+let to_proj_point_c (k:curve) (p:aff_point_c k) : proj_point_c k =
+  let px, py = p in
+  k.prime_lemma ();
+  Lib.NatMod.lemma_div_mod_prime_one #k.prime px;
+  Lib.NatMod.lemma_div_mod_prime_one #k.prime py;
+  to_proj_point k p
 
 
 let point_negate (k:curve) (p:proj_point k) : proj_point k =
