specs/ecc/Spec.EC.Projective.Lemmas.fsti
@@ -20,17 +20,21 @@ val lemma_aff_is_point_at_inf: k:curve -> p:proj_point k ->
     is_aff_point_at_inf k (to_aff_point k p) == (pz = 0 || (px = 0 && py = 0)))
 
 
-val lemma_proj_aff_id (k:curve) (p:aff_point k) :
-  Lemma (to_aff_point k (to_proj_point k p) == p)
+val lemma_aff_is_point_at_inf_c: k:curve -> p:proj_point_c k ->
+  Lemma (let px, py, pz = p in is_aff_point_at_inf k (to_aff_point k p) == (pz = 0))
 
 
 val to_aff_point_at_infinity_lemma: k:curve ->
-  Lemma (to_aff_point k (point_at_inf k) == aff_point_at_inf k)
+  Lemma (to_aff_point_c k (point_at_inf k) == aff_point_at_inf k)
+
+
+val lemma_proj_aff_id (k:curve) (p:aff_point_c k) :
+  Lemma (to_aff_point_c k (to_proj_point_c k p) == p)
 
 
 val to_aff_point_negate_lemma (k:curve) (p:proj_point_c k) :
   Lemma (point_inv k (point_negate k p) /\
-    to_aff_point k (point_negate k p) == aff_point_negate k (to_aff_point k p))
+    to_aff_point_c k (point_negate k p) == aff_point_negate k (to_aff_point_c k p))
 
 
 (** The point addition and doubling formulas are taken from
@@ -40,19 +44,23 @@ val to_aff_point_negate_lemma (k:curve) (p:proj_point_c k) :
 
 val to_aff_point_add_lemma_a3 (k:curve{k.coeff_a = (-3) % k.prime}) (p q:proj_point_c k) :
   Lemma (point_inv k (point_add_a3 k p q) /\
-    to_aff_point k (point_add_a3 k p q) == aff_point_add k (to_aff_point k p) (to_aff_point k q))
+    to_aff_point_c k (point_add_a3 k p q) ==
+    aff_point_add k (to_aff_point_c k p) (to_aff_point_c k q))
 
 
 val to_aff_point_double_lemma_a3 (k:curve{k.coeff_a = (-3) % k.prime}) (p:proj_point_c k) :
   Lemma (point_inv k (point_double_a3 k p) /\
-    to_aff_point k (point_double_a3 k p) == aff_point_add k (to_aff_point k p) (to_aff_point k p))
+    to_aff_point_c k (point_double_a3 k p) ==
+    aff_point_add k (to_aff_point_c k p) (to_aff_point_c k p))
 
 
 val to_aff_point_add_lemma_a0 (k:curve{k.coeff_a = 0}) (p q:proj_point_c k) :
   Lemma (point_inv k (point_add_a0 k p q) /\
-    to_aff_point k (point_add_a0 k p q) == aff_point_add k (to_aff_point k p) (to_aff_point k q))
+    to_aff_point_c k (point_add_a0 k p q) ==
+    aff_point_add k (to_aff_point_c k p) (to_aff_point_c k q))
 
 
 val to_aff_point_double_lemma_a0 (k:curve{k.coeff_a = 0}) (p:proj_point_c k) :
   Lemma (point_inv k (point_double_a0 k p) /\
-    to_aff_point k (point_double_a0 k p) == aff_point_add k (to_aff_point k p) (to_aff_point k p))
+    to_aff_point_c k (point_double_a0 k p) ==
+    aff_point_add k (to_aff_point_c k p) (to_aff_point_c k p))
